

★ UNIT-2:

• Eigen values and eigen vectors :-

- Eigen values and eigen vectors.
- Cayley - Hamilton theorem.
- Diagonalization
- Orthogonalization
- Quadratic form (or) canonical form.

Let $A = (a_{ij})$ be an $n \times n$ square matrix. A non-zero vector ' x ' is said to be a characteristic vector of ' A ' if there exists a scalar ' λ ' such that $Ax = \lambda x$ ($x \neq 0$). We say that ' x ' is Eigen vector or characteristic vector of ' A ' corresponding to the Eigen values (or) characteristic values of ' λ '.

• To find Eigen values and vectors of a matrix:

- Consider the matrix of order 3×3

$$A = \begin{bmatrix} a_{11} & a_{12} & a_{13} \\ a_{21} & a_{22} & a_{23} \\ a_{31} & a_{32} & a_{33} \end{bmatrix}$$

- Let us take λ as a scalar which is subtracted from the diagonal elements, we get characteristic matrix.

$$\text{i.e. } |A - \lambda I| = \begin{bmatrix} a_{11} - \lambda & a_{12} & a_{13} \\ a_{21} & a_{22} - \lambda & a_{23} \\ a_{31} & a_{32} & a_{33} - \lambda \end{bmatrix}$$

$$|A - \lambda I| = 0$$

- The characteristic polynomial of ' A ' is a determinant of A minus λ i.e. $|A - \lambda I|$ and is equated to 0. we get characteristic equation. i.e. $|A - \lambda I| = 0$.

- Solving the characteristic eqn we get the λ values, these values are called Eigen values or latent values or proper values.

note:

1. By using characteristic equation

$|A - \lambda I| = 0$ we have to calculate

Eigen values

2. By using matrix equation

$(A - \lambda I)x = 0$ we have to calculate

Eigen vectors.

• Find the characteristic roots of the matrix:

$$A = \begin{bmatrix} 2 & 2 & 1 \\ 1 & 3 & 1 \\ 1 & 2 & 2 \end{bmatrix}$$

The characteristic eqn of A is $|A - \lambda I| = 0$.

$$|A - \lambda I| = \begin{vmatrix} 2-\lambda & 2 & 1 \\ 1 & 3-\lambda & 1 \\ 1 & 2 & 2-\lambda \end{vmatrix}$$

$$\therefore (2-\lambda)[(3-\lambda)(2-\lambda)-2] - 2(2-\lambda-1) + [2-(3-\lambda)] = 0$$

$$\therefore (2-\lambda)[6-3\lambda-2\lambda+\lambda^2-2] - 2(1-\lambda) + (-1+\lambda) = 0$$

$$\therefore (2-\lambda)(\lambda^2-5\lambda+4) - 2+2\lambda-1+\lambda = 0$$

$$\therefore 2\lambda^2 - 10\lambda + 8 - \lambda^3 + 5\lambda^2 - 4\lambda - 3 + 3\lambda = 0$$

$$\therefore -\lambda^3 + 7\lambda^2 - 11\lambda + 5 = 0$$

$$\therefore \lambda^3 - 7\lambda^2 + 11\lambda - 5 = 0$$

using synthetic division; let $\lambda = 1$

$$\begin{array}{r|rrrr} 1 & 1 & -7 & 11 & -5 \\ & & 0 & 1 & -6 & 5 \\ \hline 1 & 1 & -6 & 5 & 0 \\ & & 0 & 1 & -5 \\ \hline 5 & 1 & -5 & 0 & \\ & & 0 & 5 & \\ \hline & 1 & 0 & & \end{array}$$

$$\therefore (\lambda-1)(\lambda-1)(\lambda-5) = 0$$

$$\lambda-1=0 \Rightarrow \lambda=1$$

$$\lambda-1=0 \Rightarrow \lambda=1$$

$$\lambda-5=0 \Rightarrow \lambda=5$$

\therefore The characteristic roots of A are $(1, 1, 5)$.

Q. Find the Eigen values corresponding to the Eigen vectors of matrix:

$$A = \begin{bmatrix} 8 & -6 & 2 \\ -6 & 7 & -4 \\ 2 & -4 & 3 \end{bmatrix}$$

Soln:

The characteristic eqn of A is $|A - \lambda I| = 0$ $|A - \lambda I| = 0$

$$|A - \lambda I| = \begin{vmatrix} 8-\lambda & -6 & 2 \\ -6 & 7-\lambda & -4 \\ 2 & -4 & 3-\lambda \end{vmatrix}$$

$$\Rightarrow (8-\lambda)[(7-\lambda)(3-\lambda)-16] + 6[-6(3-\lambda)+8] + 2[24-2(7-\lambda)] = 0$$

$$\therefore (8-\lambda)[21-7\lambda-3\lambda+\lambda^2-16] + 6(-18+6\lambda+8) + 2(24-14+2\lambda) = 0$$

$$\Rightarrow (8-\lambda)(\lambda^2-10\lambda+5) + 6(6\lambda-10) + 2(10+2\lambda) = 0$$

$$\Rightarrow 8\lambda^2 - 80\lambda + 40 - \lambda^3 + 10\lambda^2 - 5\lambda + 36\lambda - 60 + 20 + 4\lambda = 0$$

$$\Rightarrow -\lambda^3 + 18\lambda^2 - 45\lambda = 0$$

$$-\lambda[\lambda^2 - 18\lambda + 45] = 0$$

Here $-\lambda = 0$ and $\lambda^2 - 18\lambda + 45 = 0$

$$\lambda = 0$$

$$\lambda(\lambda-1)$$

$$\lambda^2 - 15\lambda - 3\lambda + 45 = 0$$

$$\lambda(\lambda-15) - 3(\lambda-15) = 0$$

$$(\lambda-15)(\lambda-3) = 0$$

$$\lambda-15=0 \text{ or } \lambda-3=0$$

$$\lambda=15 \text{ or } \lambda=3$$

The Eigen values of A are $0, 3, 15$.

To find Eigen vectors:

Eigen vector corresponding to $\lambda=0$

The matrix eqn is

$$(A - \lambda I)x = 0$$

$$(A - 0I)x = 0$$

put $\lambda=0$ in matrix $|A - \lambda I|$

$$\begin{bmatrix} 8 & -6 & 2 \\ -6 & 7 & -4 \\ 2 & -4 & 3 \end{bmatrix} \begin{bmatrix} x \\ y \\ z \end{bmatrix} = \begin{bmatrix} 0 \\ 0 \\ 0 \end{bmatrix}$$

$$8x - 6y + 2z = 0 \dots \dots \textcircled{1}$$

$$-6x + 7y - 4z = 0 \dots \dots \textcircled{2}$$

$$2x - 4y + 3z = 0 \dots \dots \textcircled{3}$$

Solving eq $\textcircled{1}$ and $\textcircled{2}$ by cross-multiplication method.

$$\begin{array}{ccc} y & z & x \\ -6 & 2 & 8 \\ 7 & -4 & -6 \end{array}$$

$$\frac{y}{24-14} = \frac{z}{-12+32} = \frac{x}{56-36}$$

$$\frac{y}{10} = \frac{z}{20} = \frac{x}{20}$$

$$x=2 \quad y=1 \quad z=2$$

The eigen vector corresponding to $\lambda=0$ is $X_1 = \begin{bmatrix} 2 \\ 1 \\ 2 \end{bmatrix}$.

Eigen vectors corresponding to $\lambda=3$

The matrix eqn is $|A - \lambda I| = 0$

$$|A - 3I| = 0$$

$$\begin{bmatrix} 5 & -6 & 2 \\ -6 & 4 & -4 \\ 2 & -4 & 0 \end{bmatrix} \begin{bmatrix} x \\ y \\ z \end{bmatrix} = \begin{bmatrix} 0 \\ 0 \\ 0 \end{bmatrix}$$

$$5x - 6y + 2z = 0 \dots \dots \textcircled{1}$$

$$-6x + 4y - 4z = 0 \dots \dots \textcircled{2}$$

$$2x - 4y = 0 \dots \dots \textcircled{3}$$

FF Solving eq ① and ② by cross-multiplication method,

$$\begin{array}{r} y \quad z \quad x \quad y \\ -6 \quad -6 \quad 2 \quad 5 \\ y \quad z \quad x \quad y \\ -6 \quad 2 \quad 5 \quad -6 \\ 4 \quad -4 \quad -6 \quad 4 \end{array}$$

$$\frac{y}{24-12} = \frac{z}{-12+20} = \frac{x}{20-36}$$

$$\frac{y}{16_2} = \frac{z}{-8_1} = \frac{x}{-16_2}$$

$$x = -2, y = -1, z = 2$$

The eigen vectors corresponding to

$$\lambda = 3 \text{ is}$$

$$X_2 = \begin{bmatrix} -2 \\ -1 \\ 2 \end{bmatrix}$$

Eigen vectors corresponding to $\lambda = 15$.

The matrix eqn is $|A - \lambda I| x = 0$

$$|A - 15I| x = 0$$

$$\begin{bmatrix} -7 & -6 & 2 \\ -6 & -8 & -4 \\ 2 & -4 & -12 \end{bmatrix} \begin{bmatrix} x \\ y \\ z \end{bmatrix} = \begin{bmatrix} 0 \\ 0 \\ 0 \end{bmatrix}$$

$$-7x - 6y + 2z = 0 \dots \dots \textcircled{1}$$

$$-6x - 8y - 4z = 0$$

$$2x - 4y - 12z = 0$$

$$* 3x + 4y + 2z = 0 \dots \dots \textcircled{2}$$

$$x - 2y - 6z = 0 \dots \dots \textcircled{3}$$

Using cross-multiplication method on eq ② & ③

$$\begin{array}{r} y \quad z \quad x \quad y \\ 4 \quad 2 \quad 3 \quad 4 \\ -2 \quad -6 \quad 1 \quad -2 \end{array}$$

$$\frac{y}{-24+4} = \frac{z}{2+12} = \frac{x}{-6-4}$$

$$\frac{y}{-20} = \frac{z}{20} = \frac{x}{-10}$$

$$x = -10, y = -2, z = 2$$

The Eigen vectors corresponding to

$$\lambda = 15 \text{ is } X_3 = \begin{bmatrix} -1 \\ -2 \\ 2 \end{bmatrix}$$

∴ The Eigen vectors corresponding to λ for given equation matrix are

$$X_1 = \begin{bmatrix} 2 \\ 1 \\ 2 \end{bmatrix} \quad X_2 = \begin{bmatrix} -2 \\ -1 \\ 2 \end{bmatrix} \quad X_3 = \begin{bmatrix} -1 \\ -2 \\ 2 \end{bmatrix}$$

• Find Eigen values and eigen vectors of the given vector matrix.

$$A = \begin{bmatrix} 6 & -2 & 2 \\ -2 & 3 & -1 \\ 2 & -1 & 3 \end{bmatrix}$$

• Soln. The characteristic eqn of A is

$$|A - \lambda I| = 0$$

$$\begin{bmatrix} 6-\lambda & -2 & 2 \\ -2 & 3-\lambda & -1 \\ 2 & -1 & 3-\lambda \end{bmatrix} = 0$$

$$\therefore (6-\lambda)[(3-\lambda)(3-\lambda)-1] + 2[2(3-\lambda) + 2[-2-2(3-\lambda)]] = 0$$

$$\therefore (6-\lambda)[\lambda^2 - 6\lambda + 9 - 1] + 2[6 - 2\lambda + 2[-2 - 6 + 2\lambda]] = 0$$

$$\therefore (6-\lambda)[\lambda^2 - 6\lambda + 8] + 2[8 - 2\lambda + 2[-8 + 2\lambda]] = 0$$

$$\therefore 6\lambda^2 - 36\lambda + 48 - \lambda^3 + 6\lambda^2 - 8\lambda + 16 + 4\lambda + 16 + 4\lambda = 0$$

$$\therefore -\lambda^3 + 12\lambda^2 - 36\lambda + 32 = 0$$

$$\therefore \lambda^3 - 12\lambda^2 + 36\lambda - 32 = 0$$

• Synthetic division:

$$\begin{array}{r|rrrr} 2 & 1 & -12 & 36 & -32 \\ & & 0 & 2 & -20 & 32 \\ \hline 2 & 1 & -10 & 16 & 0 \\ & & 0 & 2 & -16 \\ \hline 8 & 1 & -8 & 0 \\ & & 0 & 8 \\ \hline & 1 & 0 \end{array}$$

$$(\lambda-2)(\lambda-2)(\lambda-8) = 0$$

$$\lambda-2 = 0 \Rightarrow \lambda = 2$$

$$\lambda-2 = 0 \Rightarrow \lambda = 2$$

$$\lambda-8 = 0 \Rightarrow \lambda = 8$$

• The Eigen values are 2, 2, 8.

• To find Eigen vectors:

The Eigen vector corresponding to $\lambda = 2$ the matrix eqn is

$$(A - \lambda I) X = 0$$

$$(A - 2I) X = 0$$

$$\begin{bmatrix} 4 & -2 & 2 \\ -2 & 1 & -1 \\ 2 & -1 & 1 \end{bmatrix} \begin{bmatrix} x \\ y \\ z \end{bmatrix} = \begin{bmatrix} 0 \\ 0 \\ 0 \end{bmatrix}$$

$$4x - 2y + 2z = 0 \dots \dots \textcircled{1}$$

$$-2x + y - z = 0 \dots \dots \textcircled{2}$$

$$2x - y + z = 0 \dots \dots \textcircled{3}$$

Here eqn ① ② and ③ are same equations. we can apply substitution method

put $y = k_1, z = k_2$ in eq ③

$$2k_1 - k_1 + k_2 = 0$$

$$\Rightarrow 2k_1 - k_1 + k_2 = 0$$

$$\boxed{x = \frac{k_1 - k_2}{2}}$$

The eigen vectors corresponding to

$$\lambda = 2 \text{ is}$$

$$X = \begin{bmatrix} \frac{k_1 - k_2}{2} \\ k_1 \\ k_2 \end{bmatrix} = k_1 \begin{bmatrix} \frac{1}{2} \\ 1 \\ 0 \end{bmatrix} + k_2 \begin{bmatrix} -\frac{1}{2} \\ 0 \\ 1 \end{bmatrix}$$

The Eigen value corresponding to

$$\lambda = 8$$

The matrix eqn is $(A - \lambda I)x = 0$

$$|A - 8I| x = 0$$

$$\begin{bmatrix} -2 & -2 & 2 \\ -2 & -5 & -1 \\ 2 & -1 & -5 \end{bmatrix} \begin{bmatrix} x \\ y \\ z \end{bmatrix} = \begin{bmatrix} 0 \\ 0 \\ 0 \end{bmatrix}$$

$$-2x - 2y + 2z = 0 \dots \dots \textcircled{4}$$

$$-2x - 5y - z = 0 \dots \dots \textcircled{5}$$

$$2x - y - 5z = 0 \dots \dots \textcircled{6}$$

solving eq ⑤ and ⑥ by cross multiplication method.

$$\begin{array}{r} y \quad z \quad x \quad y \\ -5 \quad -1 \quad -2 \quad -5 \\ -1 \quad -5 \quad 2 \quad -1 \end{array}$$

$$\frac{y}{25-1} = \frac{z}{-2-10} = \frac{x}{2+10}$$

$$\frac{y}{24_2} = \frac{z}{-12_1} = \frac{x}{12_1}$$

$$x = 1, y = 2, z = -1$$

The eigen vectors corresponding to

$$\lambda = 8 \text{ is}$$

$$X_3 = \begin{bmatrix} 1 \\ 2 \\ -1 \end{bmatrix}$$

The Eigen values are 2, 2, 8 and the Eigen vectors are

$$X = \begin{bmatrix} \frac{k_1 - k_2}{2} \\ k_1 \\ k_2 \end{bmatrix} = k_1 \begin{bmatrix} \frac{1}{2} \\ 1 \\ 0 \end{bmatrix} + k_2 \begin{bmatrix} -\frac{1}{2} \\ 0 \\ 1 \end{bmatrix}$$

$$X_3 = \begin{bmatrix} 1 \\ 2 \\ -1 \end{bmatrix}$$

Practice:
Find Eigen values and corresponding Eigen vectors of the matrices.

1. $\begin{bmatrix} 1 & 1 & 1 \\ 1 & 1 & 1 \\ 1 & 1 & 1 \end{bmatrix}$ (2) $\begin{bmatrix} 2 & 2 & 0 \\ 2 & 5 & 0 \\ 0 & 0 & 3 \end{bmatrix}$

(3) $\begin{bmatrix} 1 & 0 & -1 \\ 1 & 2 & 1 \\ 2 & 2 & 3 \end{bmatrix}$ (4) $\begin{bmatrix} 1 & 1 & 3 \\ 1 & 5 & 1 \\ 3 & 1 & 1 \end{bmatrix}$

• DIAGONALIZATION : of a matrix :-

A matrix 'A' is diagonalizable if there exists an invertible matrix 'P' such that $P^{-1}AP = D$ then D is called the 'diagonal matrix'.

• Working rule :

Step 1: Find Eigen values

Step 2: Find Eigen vectors

Step 3: Write modal matrix 'P'.

i.e $P = [X_1 X_2 X_3]$

Step 4: Find the inverse of P.

[If given matrix is symmetric, we can write $P^{-1} = P^T$]

-If given matrix is not symmetric, we have to find P^{-1} value i.e $P^{-1} = \frac{1}{|P|} \text{Adj}(P)$

Step 5: Check diagonalization. i.e

$P^{-1}AP = D$

Q1. Determine the modal matrix 'P' for

$A = \begin{bmatrix} 1 & 1 & 3 \\ 1 & 5 & 1 \\ 3 & 5 & 1 \end{bmatrix}$ add hence diagonalize 'A'.

• Solⁿ: The characteristic eqn for A is

$|A - \lambda I| = 0$

$|A - \lambda I| = \begin{vmatrix} 1-\lambda & 1 & 3 \\ 1 & 5-\lambda & 1 \\ 3 & 1 & 1-\lambda \end{vmatrix}$

$\therefore (1-\lambda) [(5-\lambda)(1-\lambda) - 1] - 1[(1-\lambda)3] + 3[1 - 3(5-\lambda)] = 0$

$(1-\lambda)(5-\lambda-\lambda^2-1) - (3-3\lambda)$

$+ 3(1-15+3\lambda) = 0$

$(1-\lambda)(\lambda^2-6\lambda-4) - 3+3\lambda+3(-14+3\lambda)$

$\lambda^2-6\lambda-4-\lambda^3+6\lambda^2+4\lambda-3+3\lambda-42-9\lambda$

$\therefore -\lambda^3+7\lambda^2-36=0$

$\therefore \lambda^3-7\lambda^2+36=0 \quad (\lambda+2)(\lambda-3)(\lambda-6)=0$

$\therefore \lambda_1 = -2 \quad \lambda_2 = 6 \quad \lambda_3 = 3$

\therefore The Eigen values for the matrix A is are (-2, 6 and 3).

The Eigen vectors:

Corresponding to $\lambda = -2$

The matrix eqn is $|A - \lambda I|X = 0$

$\therefore |A + 2I|X = 0$

$\begin{bmatrix} 3 & 1 & 3 \\ 1 & 7 & 1 \\ 3 & 1 & 3 \end{bmatrix} \begin{bmatrix} x \\ y \\ z \end{bmatrix} = \begin{bmatrix} 0 \\ 0 \\ 0 \end{bmatrix}$

$3x + y + 3z = 0 \dots \textcircled{1}$

$x + 7y + z = 0 \dots \textcircled{2}$

$3x + y + 3z = 0 \dots \textcircled{3}$

Solving eq (1) and (2) by cross multiplication method.

$y \quad z \quad x \quad y$

$7 \quad 3 \quad 3 \quad 31$

$7 \quad 1 \quad 1 \quad 7$

$\frac{y}{1-21} = \frac{z}{3-3} = \frac{x}{21-1}$

$\frac{y}{-20} = \frac{z}{0} = \frac{x}{20}$

$\therefore x = 1 \quad y = -1 \quad z = 0$

$X_1 = \begin{bmatrix} 1 \\ -1 \\ 0 \end{bmatrix}$

• corresponding to $\lambda = 6$

The matrix eqn is $|A - 6I|X = 0$

$\begin{bmatrix} -5 & 1 & 3 \\ 1 & -1 & 1 \\ 3 & 1 & -5 \end{bmatrix} \begin{bmatrix} x \\ y \\ z \end{bmatrix} = \begin{bmatrix} 0 \\ 0 \\ 0 \end{bmatrix}$

$-5x + y + 3z = 0 \dots \textcircled{4}$

$x - y - z = 0 \dots \textcircled{5}$

$3x + y - 5z = 0 \dots \textcircled{6}$

Solving eq (4) and (5) by cross multiplication method.

$y \quad z \quad x \quad y$

$1 \quad 3 \quad -5 \quad 1$

$-1 \quad -1 \quad 1 \quad -1$

$\frac{y}{-1+3} = \frac{z}{3-5} = \frac{x}{5-1}$

$\frac{y}{2} = \frac{z}{-2} = \frac{x}{4}$

$x = 21 \quad y = 0 \quad z = -2$

$X_2 = \begin{bmatrix} 1 \\ 0 \\ -2 \end{bmatrix}$

• Corresponding to $\lambda = 3$

The matrix eqn is $|A - 3I|X = 0$

$\begin{bmatrix} -2 & 1 & 3 \\ 1 & 2 & 1 \\ 3 & 1 & -2 \end{bmatrix} \begin{bmatrix} x \\ y \\ z \end{bmatrix} = \begin{bmatrix} 0 \\ 0 \\ 0 \end{bmatrix}$

$-2x + y + 3z = 0 \dots \textcircled{7}$

$x + 2y + z = 0 \dots \textcircled{8}$

$3x + y - 2z = 0 \dots \textcircled{9}$

Solving eq (7) and (8) by cross multiplication method.

$y \quad z \quad x \quad y$

$1 \quad 3 \quad -2 \quad 1$

$2 \quad 1 \quad 1 \quad 2$

$\frac{y}{1-6} = \frac{z}{3+2} = \frac{x}{-4-1}$

$\frac{y}{-5} = \frac{z}{5} = \frac{x}{-5}$

$X_3 = \begin{bmatrix} 1 \\ -1 \\ 1 \end{bmatrix}$

The modal matrix $P = [X_1 X_2 X_3]$

$P = \begin{bmatrix} 1 & 1 & 1 \\ -1 & 0 & -1 \\ 0 & -2 & 1 \end{bmatrix}$

• Find P^{-1} :

Given matrix $A = \begin{bmatrix} 1 & 1 & 3 \\ 1 & 5 & 1 \\ 3 & 1 & 1 \end{bmatrix}$

$A^T = \begin{bmatrix} 1 & 1 & 3 \\ 1 & 5 & 1 \\ 3 & 1 & 1 \end{bmatrix}$

$\therefore A = A^T$ The given matrix is a symmetric matrix.

Now $P^{-1} = P^T$... ($\because A$ is symmetric matrix)

$P^{-1} = P^T$

Now $P^T = \begin{bmatrix} 1 & -1 & 0 \\ 1 & 0 & -1 \\ 0 & -2 & 1 \end{bmatrix}$

• check diagonalization:

Now $P^{-1}AP = P^TAP$

$= \begin{bmatrix} 1 & -1 & 0 \\ -1 & 1 & 1 \\ 1 & 1 & 2 \end{bmatrix} \begin{bmatrix} 1 & 1 & 3 \\ 1 & 5 & 1 \\ 3 & 1 & 1 \end{bmatrix} \begin{bmatrix} 1 & -1 & 1 \\ -1 & -1 & 1 \\ 0 & 1 & 2 \end{bmatrix}$

$= \begin{bmatrix} -2 & 0 & 0 \\ 0 & 3 & 0 \\ 0 & 0 & 6 \end{bmatrix} = D$

\therefore The diagonal matrix of A is

$D = \begin{bmatrix} -2 & 0 & 0 \\ 0 & 3 & 0 \\ 0 & 0 & 6 \end{bmatrix}$

• orthogonal reduction of real symmetric matrix.

Step 1: Eigen values

Step 2: Eigen vectors

Step 3: Normalized eigen vectors

$$\text{i.e. } \frac{x_1}{\|x_1\|}, \frac{x_2}{\|x_2\|}, \frac{x_3}{\|x_3\|}$$

$$\text{where } \|x\| = \sqrt{x^2 + y^2 + z^2}$$

Step 4: Write modal matrix

$$P = \begin{bmatrix} \frac{x_1}{\|x_1\|} & \frac{x_2}{\|x_2\|} & \frac{x_3}{\|x_3\|} \end{bmatrix}$$

Step 5: Find P^{-1}

Here given matrix is real symmetric matrix. So we can write

$$P^{-1} = P^T$$

Step 6: Check diagonalization

$$D = P^{-1}AP$$

Q. Diagonalize the matrix where A

$$A = \begin{bmatrix} 7 & 4 & 4 \\ 4 & 8 & 1 \\ -4 & 1 & 8 \end{bmatrix} \quad \begin{bmatrix} 2 & 0 & 4 \\ 0 & 6 & 0 \\ 4 & 0 & 2 \end{bmatrix}$$

• Soln: The characteristic eqn is

$$|A - \lambda I| = 0$$

$$\therefore \begin{vmatrix} 2-\lambda & 0 & 4 \\ 0 & 6-\lambda & 0 \\ 4 & 0 & 2-\lambda \end{vmatrix} = |A - \lambda I| = 0$$

$$\therefore (2-\lambda)[(6-\lambda)(2-\lambda)] + 4[-4(6-\lambda)] = 0$$

$$\therefore (2-\lambda)(12 - 6\lambda - 2\lambda + \lambda^2) + 4(-24 + 4\lambda) = 0$$

$$\therefore (2-\lambda)(\lambda^2 - 8\lambda + 12) - 96 + 16\lambda = 0$$

$$\therefore 2\lambda^2 - 16\lambda + 24 - \lambda^3 + 8\lambda^2 - 12\lambda - 96 + 16\lambda = 0$$

$$\therefore -\lambda^3 + 10\lambda^2 - 12\lambda - 72 = 0$$

$$\therefore \lambda^3 - 10\lambda^2 + 12\lambda + 72 = 0$$

$$\lambda = -2, \lambda = 6, \lambda = 6$$

The eigen vectors for $\lambda = -2$ is:

The characteristic eqn is

$$|A + 2I|x = 0$$

$$\begin{bmatrix} 4 & 0 & 4 \\ 0 & 8 & 0 \\ 4 & 0 & 4 \end{bmatrix} \begin{bmatrix} x \\ y \\ z \end{bmatrix} = \begin{bmatrix} 0 \\ 0 \\ 0 \end{bmatrix}$$

$$4x + 4z = 0$$

$$x + z = 0 \quad \text{--- (1)}$$

$$8y = 0$$

$$y = 0 \quad \text{--- (2)}$$

$$4x + 4z = 0$$

$$x + z = 0 \quad \text{--- (3)}$$

$$\text{put } z = -x \text{ in eq (1)}$$

$$\begin{aligned} x &= -k \\ y &= 0 \\ z &= k \end{aligned} \quad X_1 = \begin{bmatrix} -k \\ 0 \\ k \end{bmatrix} = k \begin{bmatrix} -1 \\ 0 \\ 1 \end{bmatrix}$$

The eigen vectors for $\lambda = 6$ is:

The characteristic eqn $|A - 6I|x = 0$

$$\begin{bmatrix} -4 & 0 & 4 \\ 0 & 0 & 0 \\ 4 & 0 & -4 \end{bmatrix} \begin{bmatrix} x \\ y \\ z \end{bmatrix} = \begin{bmatrix} 0 \\ 0 \\ 0 \end{bmatrix}$$

$$-4x + 4z = 0$$

$$x - z = 0 \quad \text{--- (1)}$$

$$x = z \quad \text{--- (2)}$$

$$4x - 4z = 0$$

$$x - z = 0 \quad \text{--- (3)}$$

$$x = z \quad \text{--- (4)}$$

$$\text{put } x = z = k$$

$$\therefore x = k \quad y = 0$$

$$z = k$$

$$X_2 = \begin{bmatrix} k \\ 0 \\ k \end{bmatrix} = k \begin{bmatrix} 1 \\ 0 \\ 1 \end{bmatrix}$$

$$X_3 = k_2 \begin{bmatrix} 0 \\ 1 \\ 0 \end{bmatrix} \quad \text{put } y = k_2$$

$$X_1 = \begin{bmatrix} -1 \\ 0 \\ 1 \end{bmatrix} \quad X_2 = \begin{bmatrix} 1 \\ 0 \\ 1 \end{bmatrix} \quad X_3 = \begin{bmatrix} 0 \\ 1 \\ 0 \end{bmatrix}$$

$$\|X_1\| = \sqrt{(-1)^2 + (1)^2} = \sqrt{2}$$

$$\|X_2\| = \sqrt{(1)^2 + (1)^2} = \sqrt{2}$$

$$\|X_3\| = \sqrt{0^2 + (1)^2 + 0^2} = \sqrt{1} = 1$$

$$\frac{X_1}{\|X_1\|} = \begin{bmatrix} -1/\sqrt{2} \\ 0 \\ 1/\sqrt{2} \end{bmatrix}$$

$$\frac{X_2}{\|X_2\|} = \begin{bmatrix} 1/\sqrt{2} \\ 0 \\ 1/\sqrt{2} \end{bmatrix}$$

$$\frac{X_3}{\|X_3\|} = \begin{bmatrix} 0 \\ 1 \\ 0 \end{bmatrix}$$

• We write the modal matrix P.

$$P = \begin{bmatrix} \frac{x_1}{\|x_1\|} & \frac{x_2}{\|x_2\|} & \frac{x_3}{\|x_3\|} \end{bmatrix}$$

$$P = \begin{bmatrix} -1/\sqrt{2} & 1/\sqrt{2} & 0 \\ 0 & 0 & 1 \\ 1/\sqrt{2} & 1/\sqrt{2} & 0 \end{bmatrix}$$

Matrix A is symmetric

$$\therefore A^{-1} = A^T$$

$$\text{similarly } P^{-1} = P^T$$

$$P^{-1} = P^T = \begin{bmatrix} -1/\sqrt{2} & 0 & 1/\sqrt{2} \\ 1/\sqrt{2} & 0 & 1/\sqrt{2} \\ 0 & 1 & 0 \end{bmatrix}$$

checking diagonalization:

$$D = P^{-1}AP$$

$$= \begin{bmatrix} -1/\sqrt{2} & 0 & 1/\sqrt{2} \\ 1/\sqrt{2} & 0 & 1/\sqrt{2} \\ 0 & 1 & 0 \end{bmatrix} \begin{bmatrix} 2 & 0 & 4 \\ 0 & 6 & 0 \\ 4 & 0 & 2 \end{bmatrix}$$

$$= \begin{bmatrix} -1/\sqrt{2} & 1/\sqrt{2} & 0 \\ 0 & 0 & 1 \\ 1/\sqrt{2} & 1/\sqrt{2} & 0 \end{bmatrix}$$

$$D = \begin{bmatrix} -2 & 0 & 0 \\ 0 & 6 & 0 \\ 0 & 0 & 6 \end{bmatrix}$$

* Caley Hamilton theorem:

Every square matrix satisfies its own characteristic equation.

Q. Verify Caley Hamilton theorem

$$\text{for the matrix } A = \begin{bmatrix} 8 & -8 & 2 \\ 4 & -3 & -2 \\ 3 & -4 & 1 \end{bmatrix}$$

• Soln:

• Given matrix

$$A = \begin{bmatrix} 8 & -8 & 2 \\ 4 & -3 & -2 \\ 3 & -4 & 1 \end{bmatrix}$$

The characteristic eqn of matrix A

$$|A - \lambda I| = 0$$

$$\therefore \begin{vmatrix} 8-\lambda & -8 & 2 \\ 4 & -3-\lambda & -2 \\ 3 & -4 & 1-\lambda \end{vmatrix} = 0$$

$$\Rightarrow (8-\lambda)[(-3-\lambda)(1-\lambda) - 8] + 8[4(1-\lambda) + 6] + 2[-16 - 3(-3-\lambda)] = 0$$

$$\Rightarrow (8-\lambda)(-3-\lambda)(1-\lambda) + 8(4-4\lambda+6) + 2(-16+9+3\lambda) = 0$$

$$\Rightarrow (8-\lambda)(\lambda^2+2\lambda-11) + 8(-4\lambda+10) + 2(3\lambda-7) = 0$$

$$\Rightarrow 8\lambda^2 + 16\lambda - 88 - \lambda^3 - 2\lambda + 11\lambda - 24\lambda + 80 + 6\lambda - 14 = 0$$

$$\Rightarrow -\lambda^3 + 6\lambda^2 + \lambda - 22 = 0$$

$$\lambda^3 - 6\lambda^2 - \lambda + 22 = 0$$

By Caley Hamilton theorem,

$$\text{put } \lambda = A$$

$$\therefore A^3 - 6A^2 - A + 22I = 0$$

is the characteristic equation.

$$A^2 = \begin{bmatrix} 38 & -48 & 34 \\ 14 & -15 & 12 \\ 11 & -16 & 15 \end{bmatrix}$$

$$A^3 = \begin{bmatrix} 214 & -296 & 206 \\ 88 & -115 & 70 \\ 69 & -100 & 69 \end{bmatrix}$$

$$6A^2 = \begin{bmatrix} 228 & -288 & 204 \\ 84 & -90 & 72 \\ 66 & -96 & 90 \end{bmatrix}$$

Substituting them in characteristic eqn

$$A^3 - 6A^2 - A + 22I = 0$$

$$\begin{bmatrix} 214 & -296 & 206 \\ 88 & -115 & 70 \\ 69 & -100 & 69 \end{bmatrix} - \begin{bmatrix} 228 & -288 & 204 \\ 84 & -90 & 72 \\ 66 & -96 & 90 \end{bmatrix}$$

$$= \begin{bmatrix} 8 & -8 & 2 \\ 4 & -3 & -2 \\ 3 & -4 & 1 \end{bmatrix} + \begin{bmatrix} 22 & 0 & 0 \\ 0 & 22 & 0 \\ 0 & 0 & 22 \end{bmatrix} = 0$$

$$\therefore \begin{bmatrix} 0 & 0 & 0 \\ 0 & 0 & 0 \\ 0 & 0 & 0 \end{bmatrix} = 0$$

\therefore The matrix A satisfies its characteristic equation.
Hence, the Cayley Hamilton theorem is proved.

• Find A^{-1} :-

By using eqn ①

$$A^3 - 6A^2 - A + 22I = 0$$

Multiplying the eqn ① by A^{-1} .

$$A^{-1}[A^3 - 6A^2 - A + 22I] = 0A^{-1} = 0$$

$$\therefore A^2 - 6A - I + 22A^{-1} = 0$$

$$22A^{-1} = I - A^2 + 6A$$

$$A^{-1} = \frac{1}{22} [I - A^2 + 6A]$$

$$A^{-1} = \frac{1}{22} \left\{ \begin{bmatrix} 1 & 0 & 0 \\ 0 & 1 & 0 \\ 0 & 0 & 1 \end{bmatrix} - \begin{bmatrix} 32 & -48 & 34 \\ 14 & -15 & 12 \\ 11 & -16 & 15 \end{bmatrix} + \begin{bmatrix} 48 & -48 & 12 \\ 24 & -18 & -12 \\ 18 & -24 & 6 \end{bmatrix} \right\}$$

$$A^{-1} = \frac{1}{22} \left\{ \begin{bmatrix} 1-32+48 & 0+48-48 & 0-34+12 \\ 0+14+24 & 1+15-18 & 0-12-12 \\ 0-11+18 & 0+16-24 & 1+15-6 \end{bmatrix} \right\}$$

$$A^{-1} = \frac{1}{22} \begin{bmatrix} 17 & 0 & -22 \\ 38 & -7 & -24 \\ 7 & -8 & 8 \end{bmatrix}$$

• Verify Cayley-Hamilton theorem of $A = \begin{bmatrix} 1 & 2 & -1 \\ 2 & 1 & -2 \\ 2 & -2 & 1 \end{bmatrix}$ and find A^4 .

• Solⁿ: The characteristic eqn is

$$|A - \lambda I| = 0$$

$$\begin{vmatrix} 1-\lambda & 2 & -1 \\ 2 & 1-\lambda & -2 \\ 2 & -2 & 1-\lambda \end{vmatrix} = 0$$

$$\therefore (1-\lambda)[(1-\lambda)(1-\lambda)-4] - 2[2(1-\lambda)+4] - \{[-4-2(1-\lambda)]\} = 0$$

$$\Rightarrow (1-\lambda)(1-\lambda-\lambda+\lambda^2-4) - 2(2-2\lambda+4) - (-4-2+2\lambda) = 0$$

$$\Rightarrow (1-\lambda)(\lambda^2-2\lambda-3) - 2(-2\lambda+6) + 6-2\lambda = 0$$

$$\Rightarrow \lambda^2 - 2\lambda - 3 - \lambda^3 + 2\lambda^2 + 3\lambda + 4\lambda - 12 + 6 - 2\lambda = 0$$

$$\Rightarrow -\lambda^3 + 3\lambda^2 + 3\lambda - 9 = 0$$

$$\Rightarrow \lambda^3 - 3\lambda^2 - 3\lambda + 9 = 0$$

By Cayley-Hamilton theorem, put $\lambda = A$.

$$A^3 - 3A^2 - 3A + 9I = 0 \quad \text{--- ①}$$

$$A^3 = \begin{bmatrix} 3 & 24 & -21 \\ 6 & 21 & -24 \\ 6 & -6 & 3 \end{bmatrix}$$

$$A^2 = \begin{bmatrix} 3 & 6 & -6 \\ 0 & 9 & -6 \\ 0 & 0 & 3 \end{bmatrix}$$

$$3A^2 = \begin{bmatrix} 9 & 18 & -18 \\ 0 & 27 & -18 \\ 0 & 0 & 9 \end{bmatrix}$$

$$3A = \begin{bmatrix} 3 & 6 & -3 \\ 6 & 3 & -6 \\ 6 & -6 & 3 \end{bmatrix}$$

Substitute these values in eqn ①.

$$\begin{bmatrix} 3 & 24 & -21 \\ 6 & 21 & -24 \\ 6 & -6 & 3 \end{bmatrix} - \begin{bmatrix} 9 & 18 & -18 \\ 0 & 27 & -18 \\ 0 & 0 & 9 \end{bmatrix} =$$

$$\begin{bmatrix} 3 & 6 & -3 \\ 6 & 3 & -6 \\ 6 & -6 & 3 \end{bmatrix} + \begin{bmatrix} 9 & 0 & 0 \\ 0 & 9 & 0 \\ 0 & 0 & 9 \end{bmatrix} = 0$$

$$\begin{bmatrix} 3-9+9 & 24-18-6+0 & -21+18+3+0 \\ 6-0-6+0 & 21-27-3+9 & -24+18+6+0 \\ 6-0-6+0 & -6+6+0-0 & 3-9-3+9 \end{bmatrix}$$

$$= \begin{bmatrix} 0 & 0 & 0 \\ 0 & 0 & 0 \\ 0 & 0 & 0 \end{bmatrix} = 0$$

\therefore Cayley-Hamilton theorem is verified.

$$\text{Now } A^4 = \begin{bmatrix} 9 & 72 & -72 \\ 0 & 81 & -72 \\ 0 & 0 & 9 \end{bmatrix}$$

using eqn ①

$$A^3 - 3A^2 - 3A + 9I = 0$$

Multiplying both sides with A

$$A^4 - 3A^3 - 3A^2 + 9A = 0$$

$$A^4 = 3A^3 + 3A^2 - 9A$$

$$A^4 = 3 \begin{bmatrix} 3 & 24 & -21 \\ 6 & 21 & -24 \\ 6 & -6 & 3 \end{bmatrix} + 3 \begin{bmatrix} 3 & 6 & -6 \\ 0 & 9 & -6 \\ 0 & 0 & 3 \end{bmatrix}$$

$$= \begin{bmatrix} 9 & 0 & 0 \\ 0 & 9 & 0 \\ 0 & 0 & 9 \end{bmatrix} - 9 \begin{bmatrix} 1 & 2 & -1 \\ 2 & 1 & -2 \\ 2 & -2 & 1 \end{bmatrix}$$

$$A^4 = \begin{bmatrix} 9+9-9 & 72+18-18 & -63-18+9 \\ 18+0-18 & 63+27-9 & -72-18+18 \\ 18+0-18 & -18+0+18 & 9+9-9 \end{bmatrix}$$

$$A^4 = \begin{bmatrix} 9 & 72 & -72 \\ 0 & 81 & -72 \\ 0 & 0 & 9 \end{bmatrix} //$$

Q. If $A = \begin{bmatrix} 2 & 1 & 1 \\ 0 & 1 & 0 \\ 1 & 1 & 2 \end{bmatrix}$ find the value of matrix

$$A^3 - 5A^2 + 7A - 3A^5 + A^4 - 5A^3 + 8A^2 - 2A + I = 0.$$

• Soln:

The characteristic eqn of matrix A is $|A - \lambda I| = 0$

$$\therefore \begin{vmatrix} 2-\lambda & 1 & 1 \\ 0 & 1-\lambda & 0 \\ 1 & 1 & 2-\lambda \end{vmatrix} = 0$$

$$\Rightarrow (2-\lambda)[(1-\lambda)(2-\lambda)] + 1(-1+\lambda) = 0$$

$$\Rightarrow (2-\lambda)(2-\lambda-2\lambda+\lambda^2) - 1+\lambda = 0$$

$$\Rightarrow 4 - 4\lambda + 2\lambda^2 - 2\lambda + \lambda^2 - 1 + \lambda = 0$$

$$\Rightarrow \lambda^3 + 3\lambda^2 - 5\lambda - 1 = 0$$

$$\Rightarrow (2-\lambda)(\lambda^2 - 3\lambda + 2) - 1 + \lambda = 0$$

$$2\lambda^2 - 6\lambda + 4 - \lambda^3 + 3\lambda^2 - 2\lambda - 1 + \lambda = 0$$

$$\Rightarrow -\lambda^3 + 5\lambda^2 - 7\lambda + 3 = 0$$

$$\Rightarrow \lambda^3 - 5\lambda^2 + 7\lambda - 3 = 0$$

By Cayley Hamilton theorem:

$$\text{put } \lambda = A$$

$$A^3 - 5A^2 + 7A - 3 = 0 \dots \textcircled{1}$$

So,

$$A^3 - 5A^2 + 7A - 3A^5 + A^4 - 5A^3 + 8A^2 - 2A + I$$

$$= A^5[A^3 - 5A^2 + 7A - 3I] + A^4 - 5A^3 + 8A^2 - 2A + I$$

$$= A^5(0) + A^4 - 5A^3 + 7A^2 + A^2 - 3A + A + I$$

$$= A(A^4 - 5A^3 + 7A^2 - 3A) + A^2 + A + I$$

$$= A(A^3 - 5A^2 + 7A - 3) + A^2 + A + I$$

$$= A(0) + A^2 + A + I$$

$$= A^2 + A + I$$

$$A^2 = \begin{bmatrix} 5 & 4 & 4 \\ 0 & 1 & 0 \\ 4 & 4 & 5 \end{bmatrix}$$

$$A^2 + A + I = \begin{bmatrix} 5 & 4 & 4 \\ 0 & 1 & 0 \\ 4 & 4 & 5 \end{bmatrix} + \begin{bmatrix} 2 & 1 & 1 \\ 0 & 1 & 0 \\ 1 & 1 & 2 \end{bmatrix} + \begin{bmatrix} 1 & 0 & 0 \\ 0 & 1 & 0 \\ 0 & 0 & 1 \end{bmatrix}$$

$$= \begin{bmatrix} 8 & 5 & 5 \\ 0 & 3 & 0 \\ 5 & 5 & 8 \end{bmatrix}$$

• Quadratic form:

\Rightarrow Quadratic form notation.

$$Q = a_{11}x_1^2 + a_{12}x_1x_2 + a_{13}x_1x_3 + \dots + a_{2n}x_1x_n$$

$$+ a_{21}x_2x_1 + a_{22}x_2^2 + a_{23}x_2x_3 + \dots + a_{2n}x_2x_n$$

$$+ \dots + a_{n1}x_nx_1 + a_{n2}x_nx_2 + a_{n3}x_nx_3 + \dots + a_{nn}x_n^2$$

$$Q.f = \sum_{i=1}^n \sum_{j=1}^n a_{ij} x_i x_j$$

where a_{ij} are the co-efficients (constants).

\rightarrow Every quadratic form in n variables can be expressed in the form

$$X^T A X.$$

where, A is symmetric matrix
 x is variable matrix.

The quadratic form are 5 types:

1. Positive definite: All the eigen values are positive.

eg: 1, 2, 3.

2. Positive semi-definite: At least one eigen value is zero and remaining all are positive. eg: 0, 1, 2

3. Negative definite: All the eigen values are negative.

eg: -1, -2, -3.

4. Negative semi-definite: At least one eigen value is zero remaining all are negative.

eg: 0, -1, -2.

5. Indefinite: If the eigen values are positive and negative.

eg: -1, 2, -3.

• Write the quadratic form into matrix form:

x	x	y	z	x	x	y	z
x	x^2	xy		x	x^2	xy	xz
y	yx	y^2		y	yx	y^2	yz
			z		zx	zy	z^2

1. Write the matrix of the given quadratic form is

$$x^2 + y^2 + 2xy + 4yz + 2zx$$

Sol: Given, $Q.f = x^2 + y^2 + 2xy + 4yz + 2zx$

$$= x^2 + y^2 + xy + xy + 2yz + 2yz + zx + zx$$

x	x	y	z	x	x	y	z
x	1	1	1	$A = \begin{bmatrix} 1 & 1 & 1 \\ 1 & 1 & 2 \\ 1 & 2 & 0 \end{bmatrix}$			
y	1	1	2				
z	1	2	0				

• Write the matrix of a given quadratic form

$$ax^2 + by^2 + cz^2 + 2hxy + 2gyz + 2fzx$$

• Soln: Given, $Q.f =$

$$ax^2 + by^2 + cz^2 + 2hxy + 2gyz + 2fzx$$

$$= ax^2 + by^2 + cz^2 + hxy + hxy + gyz + gyz + fzx + fzx$$

x	x	y	z	x	x	y	z
x	a	h	f	$A = \begin{bmatrix} a & h & f \\ h & b & g \\ f & g & c \end{bmatrix}$			
y	h	b	g				
z	f	g	c				

Write the matrix of the given quadratic form

$$x_1^2 + x_2^2 - x_3^2 - 2x_1x_2 - 3x_2x_3$$

Solⁿ: Given:

$$Q.F = x_1^2 + x_2^2 - x_3^2 - 2x_1x_2 - 3x_2x_3$$

$$x_1^2 + x_2^2 - x_3^2 - x_1x_2 - x_1x_2 - \frac{3}{2}x_2x_3 - \frac{3}{2}x_2x_3$$

x	x_1	x_2	x_3
x_1	1	-1	0
x_2	-1	1	-3/2
x_3	0	-3/2	-1

$$A = \begin{bmatrix} 1 & -1 & 0 \\ -1 & 1 & -3/2 \\ 0 & -3/2 & -1 \end{bmatrix}$$

• Change the given matrix into quadratic form.

$$A = \begin{bmatrix} 1 & 2 & 3 \\ 2 & -1 & 0 \\ 3 & 0 & 2 \end{bmatrix}$$

• Given: $A = \begin{bmatrix} 1 & 2 & 3 \\ 2 & -1 & 0 \\ 3 & 0 & 2 \end{bmatrix}_{3 \times 3}$

Let us consider,

$$X = \begin{bmatrix} x_1 \\ x_2 \\ x_3 \end{bmatrix} \Rightarrow X^T = [x_1 \ x_2 \ x_3]$$

Now, $X^TAX = [x_1 \ x_2 \ x_3]$

$$\begin{bmatrix} 1 & 2 & 3 \\ 2 & -1 & 0 \\ 3 & 0 & 2 \end{bmatrix} \begin{bmatrix} x_1 \\ x_2 \\ x_3 \end{bmatrix}$$

$$= [x_1 + 2x_2 + 3x_3 \quad 2x_1 - x_2 + 3x_3 \quad 3x_1 + 2x_3]$$

$$\begin{bmatrix} x_1 \\ x_2 \\ x_3 \end{bmatrix}$$

$$= x_1(x_1 + 2x_2 + 3x_3) + x_2(2x_1 - x_2) +$$

$$x_3(3x_1 + 2x_3)$$

$$= x_1^2 + 2x_1x_2 + 3x_1x_3 + 2x_2x_1 - x_2^2 - x_3^2 + 3x_2x_3 + 2x_3^2$$

$$Q.F: x_1^2 - x_2^2 + 2x_3^2 + 4x_1x_2 + 6x_1x_3$$

• Change the given matrix into quadratic form:

$$A = \begin{bmatrix} 1 & 2 \\ 2 & 5 \end{bmatrix}$$

• Solⁿ: Given, $A = \begin{bmatrix} 1 & 2 \\ 2 & 5 \end{bmatrix}_{2 \times 2}$

Let us consider,

$$X = \begin{bmatrix} x_1 \\ x_2 \end{bmatrix} \Rightarrow X^{-1} [x_1 \ x_2]$$

Now,

$$X^TAX = [x_1 \ x_2] \begin{bmatrix} 1 & 2 \\ 2 & 5 \end{bmatrix} \begin{bmatrix} x_1 \\ x_2 \end{bmatrix}$$

$$= [x_1 + 2x_2 \quad 2x_1 + 5x_2] \begin{bmatrix} x_1 \\ x_2 \end{bmatrix}$$

$$= x_1(x_1 + 2x_2) + x_2(2x_1 + 5x_2)$$

$$= x_1^2 + 2x_1x_2 + 2x_1x_2 + 5x_2^2$$

$$Q.F. = x_1^2 + 5x_2^2 + 4x_1x_2$$

• Reduction of Q.F. into canonical form:

Quadratic form: combination of product terms and power terms.

canonical form: only power terms

→ We can change quadratic form into canonical form by using 3 methods:

1. Orthogonalization
2. Diagonalization
3. Lagrange's reduction.

• Reduction of Q.F. into C.F. by

Orthogonalization:

• Working rule:

Step 1: Write symmetric matrix

Step 2: Find eigen values

Step 3: Find eigen vectors

Step 4: Write the modal matrix

$$P = \left[\frac{x_1}{\|x_1\|} \quad \frac{x_2}{\|x_2\|} \quad \frac{x_3}{\|x_3\|} \right]$$

Which is formed by normalized eigen vectors and D = diagonal matrix which is formed by eigen values.

Step 5: Find P^{-1} .

'P' is orthogonal matrix $[PP^T = I]$

$$\Rightarrow P^{-1} = P^T$$

Step 6: $D = P^TAP$.

Step 7: Canonical form $X^TDX = Y^TDY$

$$\text{i.e. } X^T[P^TAP]X$$

$$Y^T[P^TAP]Y \quad \text{METHOD I}$$

Q. Reduce the given quadratic form into canonical form by orthogonalization.

$$x_1^2 + 3x_2^2 + 3x_3^2 - 2x_2x_3$$

• Solⁿ: Given. $Q.F = x_1^2 + 3x_2^2 + 3x_3^2 - 2x_2x_3$

• Step I write symmetric matrix

x	x_1	x_2	x_3
x_1	1	0	0
x_2	0	3	-1
x_3	0	-1	3

$$A = \begin{bmatrix} 1 & 0 & 0 \\ 0 & 3 & -1 \\ 0 & -1 & 3 \end{bmatrix}$$

• Step 2: find eigen values

The characteristic equation is

$$|A - \lambda I| = 0$$

$$\begin{vmatrix} 1-\lambda & 0 & 0 \\ 0 & 3-\lambda & -1 \\ 0 & -1 & 3-\lambda \end{vmatrix} = 0$$

$$(1-\lambda)(3-\lambda) = 0$$

$$(1-\lambda)[(3-\lambda)^2 - 1] = 0$$

$$(1-\lambda)(9 - 6\lambda + \lambda^2 - 1) = 0$$

$$(1-\lambda)(\lambda^2 - 6\lambda + 8) = 0$$

$$\lambda^2 - 6\lambda + 8 - \lambda^3 + 6\lambda^2 - 8\lambda = 0$$

$$-\lambda^3 + 7\lambda^2 - 14\lambda + 8 = 0$$

$$\lambda^3 - 7\lambda^2 + 14\lambda - 8 = 0$$

By solving the equation we get,

$$\lambda = 1, 2, 4$$

∴ The Eigen values are 1, 2, 4.

• Step 3. To find Eigen vectors

The Eigen vectors corresponding to $\lambda = 1$

The matrix eqn is given by

$$(A - I)X = 0$$

$$\begin{bmatrix} 0 & 0 & 0 \\ 0 & 2 & -1 \\ 0 & -1 & 2 \end{bmatrix} \begin{bmatrix} x_1 \\ x_2 \\ x_3 \end{bmatrix} = \begin{bmatrix} 0 \\ 0 \\ 0 \end{bmatrix}$$

corresponding equations are

$$2x_2 - x_3 = 0 \dots \textcircled{1}$$

$$-x_2 + 2x_3 = 0 \dots \textcircled{2}$$

Solving eqⁿ ① and ② by crossmultiplication

$$\frac{x_2}{2} = \frac{x_3}{-1} = \frac{x_1}{0}$$

$$\frac{x_2}{-1} = \frac{x_3}{2} = \frac{x_1}{0}$$

$$\frac{x_1}{4-1} = \frac{x_2}{0} = \frac{x_3}{0}$$

$$\frac{x_1}{3} = \frac{x_2}{0} = \frac{x_3}{0} \quad X_1 = \begin{bmatrix} 1 \\ 0 \\ 0 \end{bmatrix}$$

The eigen vectors corresponding to $\lambda = 2$ $|A - \lambda I|X = 0$

The matrix eqn is $|A - 2I|X = 0$

$$\therefore \begin{bmatrix} -2 & 0 & 0 \\ 0 & 1 & -1 \\ 0 & -1 & 1 \end{bmatrix} \begin{bmatrix} x_1 \\ x_2 \\ x_3 \end{bmatrix} = \begin{bmatrix} 0 \\ 0 \\ 0 \end{bmatrix}$$

The corresponding eqns are

$$-2x_1 = 0$$

$$x_1 = 0 \dots \dots \textcircled{4}$$

$$x_2 - x_3 = 0$$

$$x_2 = x_3 \dots \dots \textcircled{5}$$

$$-x_2 + x_3 = 0$$

$$x_3 = x_2 \dots \dots \textcircled{3}$$

put $x_3 = K$ in eq $\textcircled{5}$

$$x_2 = x_3 = K$$

$$X_2 = \begin{bmatrix} 0 \\ K \\ K \end{bmatrix} = K \begin{bmatrix} 0 \\ 1 \\ 1 \end{bmatrix} \quad X_2 = \begin{bmatrix} 0 \\ 1 \\ 1 \end{bmatrix}$$

The eigen vectors corresponding to $\lambda = 4$

The matrix eqn is $|A - \lambda I|X = 0$

$$|A - 4I|X = 0$$

$$\begin{bmatrix} -3 & 0 & 0 \\ 0 & -1 & -1 \\ 0 & -1 & -1 \end{bmatrix} \begin{bmatrix} x_1 \\ x_2 \\ x_3 \end{bmatrix} = \begin{bmatrix} 0 \\ 0 \\ 0 \end{bmatrix}$$

The corresponding eqns are

$$-3x_1 = 0$$

$$x_1 = 0 \dots \dots \textcircled{7}$$

$$-x_2 - x_3 = 0$$

$$x_2 = -x_3 \dots \dots \textcircled{8}$$

$$-x_2 - x_3 = 0 \dots \dots \textcircled{9}$$

put $x_3 = K$ in eq $\textcircled{8}$

$$x_2 = -x_3 = -K$$

$$X_3 = \begin{bmatrix} 0 \\ K \\ -K \end{bmatrix} = K \begin{bmatrix} 0 \\ 1 \\ -1 \end{bmatrix}$$

$$X_1 = \begin{bmatrix} 1 \\ 0 \\ 0 \end{bmatrix} \quad X_2 = \begin{bmatrix} 0 \\ 1 \\ 1 \end{bmatrix} \quad X_3 = \begin{bmatrix} 0 \\ 1 \\ -1 \end{bmatrix}$$

step 3:

The normalized vectors are

$$\|X_1\| = \sqrt{0^2 + 1^2 + 1^2} = \sqrt{2}$$

$$\|X_2\| = \sqrt{1^2 + 0^2 + 0^2} = \sqrt{1} = 1$$

$$\frac{X_1}{\|X_1\|} = \begin{bmatrix} 1 \\ 0 \\ 0 \end{bmatrix}$$

$$\|X_2\| = \sqrt{0^2 + 1^2 + 1^2} = \sqrt{2}$$

$$\frac{X_2}{\|X_2\|} = \begin{bmatrix} 0 \\ 1/\sqrt{2} \\ 1/\sqrt{2} \end{bmatrix}$$

$$\|X_3\| = \sqrt{0^2 + 1^2 + (-1)^2} = \sqrt{2}$$

$$\frac{X_3}{\|X_3\|} = \begin{bmatrix} 0 \\ 1/\sqrt{2} \\ -1/\sqrt{2} \end{bmatrix}$$

Write modal matrix (step 4)

$$P = \begin{bmatrix} \frac{X_1}{\|X_1\|} & \frac{X_2}{\|X_2\|} & \frac{X_3}{\|X_3\|} \end{bmatrix}$$

$$P = \begin{bmatrix} 1 & 0 & 0 \\ 0 & 1/\sqrt{2} & 1/\sqrt{2} \\ 0 & 1/\sqrt{2} & -1/\sqrt{2} \end{bmatrix}$$

(step 5)

$\therefore P$ is orthogonal matrix $[P^T = I]$

$$\therefore P^{-1} = P^T$$

$$P^{-1} = P^T = \begin{bmatrix} 1 & 0 & 0 \\ 0 & 1/\sqrt{2} & 1/\sqrt{2} \\ 0 & 1/\sqrt{2} & -1/\sqrt{2} \end{bmatrix}$$

Step 6: $D = P^{-1}AP$

$$D = \begin{bmatrix} 1 & 0 & 0 \\ 0 & 1/\sqrt{2} & 1/\sqrt{2} \\ 0 & 1/\sqrt{2} & -1/\sqrt{2} \end{bmatrix} \begin{bmatrix} 1 & 0 & 0 \\ 0 & 3 & -1 \\ 0 & -1 & 3 \end{bmatrix} \begin{bmatrix} 1 & 0 & 0 \\ 0 & 1/\sqrt{2} & 1/\sqrt{2} \\ 0 & 1/\sqrt{2} & -1/\sqrt{2} \end{bmatrix}$$

$$D = \begin{bmatrix} 1 & 0 & 0 \\ 0 & 2 & 0 \\ 0 & 0 & 4 \end{bmatrix}$$

Hence $D = P^{-1}AP$

Step 7: Canonical Form = $Y^T D Y$

$$\text{Let } Y = \begin{bmatrix} y_1 \\ y_2 \\ y_3 \end{bmatrix} \Rightarrow Y^T = [y_1 \ y_2 \ y_3]$$

Now, $Y^T D Y =$

$$[y_1 \ y_2 \ y_3] \begin{bmatrix} 1 & 0 & 0 \\ 0 & 2 & 0 \\ 0 & 0 & 4 \end{bmatrix} \begin{bmatrix} y_1 \\ y_2 \\ y_3 \end{bmatrix}$$

$$[y_1 \ 2y_2 \ 4y_3] \begin{bmatrix} y_1 \\ y_2 \\ y_3 \end{bmatrix}$$

$$C.F = y_1^2 + 2y_2^2 + 4y_3^2 //$$

Reduce the Q.F into **METHOD II** c.F. by diagonalization.

Working rule:

Step 1: Write the symmetric matrix

Step 2: Write $A = I_m A I_n$ form.

Apply row operation in pre-factor matrix and column operation in post factor matrix.

The given matrix we can change into diagonal matrix.

$$D = P A P$$

$$D = P A P^T$$

Step 3: Canonical Form = $Y^T D Y$

Q. Reduce the quadratic equation into Canonical form by diagonalization

$$6x_1^2 + 3x_2^2 + 3x_3^2 - 4x_1x_2 - 2x_2x_3 + 4x_3x_1$$

Soln: The given quadratic eqn is

$$6x_1^2 + 3x_2^2 + 3x_3^2 - 4x_1x_2 - 2x_2x_3 + 4x_3x_1$$

Step 1: Write symmetric matrix

$$\begin{matrix} & x_1 & x_2 & x_3 \\ x_1 & 6 & -2 & 2 \\ x_2 & -2 & 3 & -1 \\ x_3 & 2 & -1 & 3 \end{matrix} \therefore A = \begin{bmatrix} 6 & -2 & 2 \\ -2 & 3 & -1 \\ 2 & -1 & 3 \end{bmatrix}$$

Step 2: Write $A = I_m A I_n$

$$A = I_3 A I_3$$

$$\begin{bmatrix} 6 & -2 & 2 \\ -2 & 3 & -1 \\ 2 & -1 & 3 \end{bmatrix} = \begin{bmatrix} 1 & 0 & 0 \\ 0 & 1 & 0 \\ 0 & 0 & 1 \end{bmatrix} A \begin{bmatrix} 1 & 0 & 0 \\ 0 & 1 & 0 \\ 0 & 0 & 1 \end{bmatrix}$$

$$R_2 \rightarrow 3R_2 + R_1, R_3 \rightarrow 3R_3 - R_1$$

$$\begin{bmatrix} 6 & -2 & 2 \\ 0 & 7 & -1 \\ 0 & -1 & 7 \end{bmatrix} = \begin{bmatrix} 1 & 0 & 0 \\ 1 & 3 & 0 \\ 0 & 0 & 3 \end{bmatrix} A \begin{bmatrix} 1 & 0 & 0 \\ 0 & 1 & 0 \\ 0 & 0 & 1 \end{bmatrix}$$

$$R_3 \rightarrow 7R_3 + R_2$$

$$\begin{bmatrix} 6 & -2 & 2 \\ 0 & 7 & -1 \\ 0 & 0 & 48 \end{bmatrix} = \begin{bmatrix} 1 & 0 & 0 \\ 1 & 3 & 0 \\ -6 & 3 & 21 \end{bmatrix} A \begin{bmatrix} 1 & 0 & 0 \\ 0 & 1 & 0 \\ 0 & 0 & 1 \end{bmatrix}$$

$$C_2 \rightarrow 3C_2 + C_1, C_3 \rightarrow 3C_3 - C_1$$

$$\begin{bmatrix} 6 & 0 & 0 \\ 0 & 21 & -3 \\ 0 & 0 & 144 \end{bmatrix} = \begin{bmatrix} 1 & 0 & 0 \\ 1 & 3 & 0 \\ -6 & 3 & 21 \end{bmatrix} A \begin{bmatrix} 1 & 0 & 0 \\ 0 & 3 & 0 \\ 0 & 0 & 3 \end{bmatrix}$$

$$\begin{bmatrix} 6 & 0 & 0 \\ 0 & 21 & -3 \\ 0 & 0 & 144 \end{bmatrix} = \begin{bmatrix} 1 & 0 & 0 \\ 1 & 3 & 0 \\ -6 & 3 & 21 \end{bmatrix} A \begin{bmatrix} 1 & 0 & 0 \\ 0 & 3 & 0 \\ 0 & 0 & 3 \end{bmatrix}$$

$$C_3 \rightarrow 7C_3 + C_2$$

$$\begin{bmatrix} 6 & 0 & 0 \\ 0 & 21 & 0 \\ 0 & 0 & 1008 \end{bmatrix} = \begin{bmatrix} 1 & 0 & 0 \\ 1 & 3 & 0 \\ -6 & 3 & 21 \end{bmatrix} A \begin{bmatrix} 1 & 0 & 0 \\ 0 & 3 & 0 \\ 0 & 0 & 21 \end{bmatrix}$$

$$D = P A Q$$

$$D = P A P^T$$

Step 3: Canonical form = $Y^T D Y$

$$\text{Let } Y = \begin{bmatrix} y_1 \\ y_2 \\ y_3 \end{bmatrix} \quad Y^T = [y_1 \ y_2 \ y_3]$$

$$\text{Now } Y^T D Y = [y_1 \ y_2 \ y_3] \begin{bmatrix} 6 & 0 & 0 \\ 0 & 21 & 0 \\ 0 & 0 & 1008 \end{bmatrix} \begin{bmatrix} y_1 \\ y_2 \\ y_3 \end{bmatrix}$$

$$= \begin{bmatrix} 6y_1 & 21y_2 & 1008y_3 \end{bmatrix} \begin{bmatrix} y_1 \\ y_2 \\ y_3 \end{bmatrix}$$

$$C.F. = 6y_1^2 + 21y_2^2 + 1008y_3^2$$

Q. Reduce the QF into C.F. By orthogonalization.

$$\begin{aligned} 1. & 5x^2 + 26y^2 + 10z^2 + 4yz + 14zx + 6xy \\ 2. & 3x^2 + 2y^2 + 3z^2 - 2xy - 2yz \\ 3. & 2x^2 + 2x_2^2 + 2x_3^2 + 2x_2x_3 \end{aligned}$$

• Diagonalization:

$$\begin{aligned} 1. & x_1^2 + 2x_2^2 + 2x_3^2 - 2x_1x_2 + 2x_1x_3 - 2x_2x_3 \\ 2. & 8x^2 - 7y^2 + 3z^2 + 12xy + 4xz - 8yz \end{aligned}$$

• Reduce QF into C.F. by Lagrange's reduction:

• Working rule:

- Step 1: Take the common terms from the product form of QF

- Step 2: Make perfect square by regrouping the terms.

- Step 3: The resulting relation gives Quadratic form.

Q1. Reduce the QF into C.F. by Lagrange's reduction.

$$x_1^2 + 2x_2^2 - 7x_3^2 - 4x_1x_2 + 8x_1x_3$$

• Soln: Given quadratic form is

$$QF = x_1^2 + 2x_2^2 - 7x_3^2 - 4x_1x_2 + 8x_1x_3$$

$$\Rightarrow x_1^2 + 2x_2^2 - 7x_3^2 - 4x_1[x_2 - 2x_3]$$

$$\Rightarrow x_1^2 - 4x_1[x_2 - 2x_3] + 2x_2^2 - 7x_3^2$$

$$\Rightarrow (x_1 - 2x_2 + 4x_3)^2 + 2x_2^2 - 7x_3^2$$

$$\Rightarrow [x_1 - 2x_2 + 4x_3]^2 + 4(x_2 - 2x_3)^2$$

$$+ 2x_2^2 - 7x_3^2$$

$$\Rightarrow [x_1 - 2x_2 + 4x_3]^2 + 2x_2^2 - 7x_3^2$$

$$- 4(x_2 - 2x_3)^2 + 2x_2^2 - 7x_3^2$$

$$\Rightarrow [x_1 - 2(x_2 - 2x_3)]^2 - 4[x_2^2 - 4x_2x_3 + 4x_3^2] + 2x_2^2 - 7x_3^2$$

$$\Rightarrow [x_1 - 2(x_2 - 2x_3)]^2 - 4x_2^2 + 16x_2x_3 - 16x_3^2 + 2x_2^2 - 7x_3^2$$

$$\Rightarrow [x_1 - 2(x_2 - 2x_3)]^2 - 2x_2^2 + 16x_2x_3 - 23x_3^2$$

$$\Rightarrow [x_1 - 2(x_2 - 2x_3)]^2 - 2[x_2^2 - 8x_2x_3 - 23x_3^2]$$

$$\Rightarrow [x_1 - 2(x_2 - 2x_3)]^2 - 2[x_2^2 - 8x_2x_3 + 16x_3^2] + 32x_3^2 - 23x_3^2$$

$$\Rightarrow [x_1 - 2(x_2 - 2x_3)]^2 - 2[x_2 - 4x_3]^2 + 9x_3^2$$

$$C.F. = [x_1 - 2(x_2 - 2x_3)]^2 - 2[x_2 - 4x_3]^2 + 9x_3^2$$

Q2. By Lagrange's reduction

transform the QF X^TAX to sum

of squares for $A = \begin{bmatrix} 1 & 2 & 4 \\ 2 & 6 & -2 \\ 4 & -2 & 18 \end{bmatrix}$

• Soln: Given matrix

$$A = \begin{bmatrix} 1 & 2 & 4 \\ 2 & 6 & -2 \\ 4 & -2 & 18 \end{bmatrix}$$

$$\text{Let } X = \begin{bmatrix} x_1 \\ x_2 \\ x_3 \end{bmatrix} \quad X^T = [x_1 \ x_2 \ x_3]$$

Now, $X^TAX =$

$$\begin{bmatrix} x_1 & x_2 & x_3 \end{bmatrix} \begin{bmatrix} 1 & 2 & 4 \\ 2 & 6 & -2 \\ 4 & -2 & 18 \end{bmatrix} \begin{bmatrix} x_1 \\ x_2 \\ x_3 \end{bmatrix}$$

$$[x_1 + 2x_2 + 4x_3 \quad 2x_1 + 6x_2 - 2x_3 \quad 4x_1 - 2x_2 + 18x_3]$$

$$\times \begin{bmatrix} x_1 \\ x_2 \\ x_3 \end{bmatrix}$$

$$= x_1(x_1 + 2x_2 + 4x_3) + x_2(2x_1 + 6x_2 - 2x_3)$$

$$+ x_3(4x_1 - 2x_2 + 18x_3)$$

$$= x_1^2 + 2x_1x_2 + 4x_1x_3 + 2x_1x_2 + 6x_2^2 - 2x_2x_3$$

$$+ 4x_1x_3 - 2x_2x_3 + 18x_3^2$$

$$= x_1^2 + 6x_2^2 + 18x_3^2 + 4x_1x_2 + 8x_1x_3 - 4x_2x_3$$

$$QF = x_1^2 + 6x_2^2 + 18x_3^2 + 4x_1x_2 + 8x_1x_3 - 4x_2x_3$$

$$\Rightarrow x_1^2 + 6x_2^2 + 18x_3^2 + 4x_1(x_2 + 2x_3) - 4x_2x_3$$

$$\Rightarrow x_1^2 + 6x_2^2 + 18x_3^2 + 4x_1(x_2 + 2x_3) - 4x_2x_3$$

$$\Rightarrow [x_1 + 2(x_2 + 2x_3)]^2 - 4(x_2 + 2x_3)^2$$

$$- 4(x_2 + 2x_3)^2 + 6x_2^2 + 18x_3^2 - 4x_2x_3$$

$$\Rightarrow [x_1 + 2(x_2 + 2x_3)]^2 - 4[x_2^2 + 4x_2x_3 + 4x_3^2]$$

$$+ 6x_2^2 + 18x_3^2 - 4x_2x_3$$

$$\Rightarrow [x_1 + 2(x_2 + 2x_3)]^2 - 4x_2^2 - 16x_2x_3 - 16x_3^2$$

$$+ 6x_2^2 + 18x_3^2 - 4x_2x_3$$

$$\Rightarrow [x_1 + 2(x_2 + 2x_3)]^2 + 2x_2^2 - 20x_2x_3$$

$$+ 2x_3^2$$

$$\Rightarrow [x_1 + 2(x_2 + 2x_3)]^2 + 2[x_2^2 - 10x_2x_3] + 2x_3^2$$

$$\Rightarrow [x_1 + 2(x_2 + 2x_3)]^2 + 2[x_2^2 - (2x_3)(5x_3) + 25x_3^2]$$

$$- 50x_3^2 + 2x_3^2$$

$$\Rightarrow [x_1 + 2(x_2 + 2x_3)]^2 + 2[x_2 - 5x_3]^2$$

$$- 48x_3^2 = C.F.$$